epfd/Epfd/PropositionalProofs.lean
@@ -22,9 +22,24 @@ variable (GST: ℕ)
 -- The message delay after GST, unknown to the processes
 variable (MsgDelay: ℕ)
 
+/-- A process `p` never crashes, i.e., `[](p ∉ crashed)`.  -/
+def never_crashes (tr: Trace Proc) (p: Proc): Prop :=
+  ∀ i: ℕ,
+    p ∉ (tr i).s.crashed
+
+/-- A process `p` never crashes, i.e., `[](p ∈ crashed)`.  -/
+def eventually_crashes (tr: Trace Proc) (p: Proc): Prop :=
+  ∃ i: ℕ,
+    p ∈ (tr i).s.crashed
+
 /--
-  A single step does not decrease the clock value.
+  Eventually, `p` never registers `q` as alive, i.e., `<>[](q ∉ alive[p])`.
   -/
+def eventually_never_alive (tr: Trace Proc) (p q: Proc): Prop :=
+  ∃ i: ℕ, ∀ k: ℕ,
+    q ∉ (tr (i + k)).s.alive[p]!
+
+/-- A single step does not decrease the clock value.  -/
 lemma clock_is_monotonic_in_one_step
     (s: ProtocolState Proc) (s': ProtocolState Proc) (a: Action Proc)
     (h_next: next_a Proc InitDelay GST MsgDelay s s' a):
@@ -40,9 +55,7 @@ lemma clock_is_monotonic_in_one_step
   | Timeout _ => unfold timeout at h_next; simp [h_next]
   | Crash _ => unfold crash at h_next; simp [h_next]
 
-/--
-  A single step does not decrease the set of the crashed processes.
-  -/
+/-- A single step does not decrease the set of the crashed processes.  -/
 lemma crashed_is_monotonic_in_one_step
     (s: ProtocolState Proc) (s': ProtocolState Proc) (a: Action Proc)
     (h_next: next_a Proc InitDelay GST MsgDelay s s' a):
@@ -85,6 +98,27 @@ lemma clock_is_monotonic_in_fair_run
     -- now just apply transitivity
     exact le_trans ik h_last_step_mono
 
+/-- The set `crashed` grows monotonically in a fair run. -/
+lemma crashed_is_monotonic_in_fair_run
+    (tr: Trace Proc)
+    (h_is_fair_run: is_fair_run Proc InitDelay GST MsgDelay tr)
+    (p: Proc) (i: ℕ) (h_p_crashed: p ∈ (tr i).s.crashed) (k: ℕ):
+      p ∈ (tr (i + k)).s.crashed := by
+  induction k with
+  | zero => exact h_p_crashed
+  | succ k ik =>
+    unfold is_fair_run at h_is_fair_run
+    rcases h_is_fair_run with ⟨ h_is_run, _ ⟩
+    unfold is_run at h_is_run
+    rcases h_is_run with ⟨ _, h_is_path ⟩
+    unfold is_path at h_is_path
+    specialize h_is_path (i + k)
+    -- apply next_does_not_decrease_clock to the last step
+    have h_last_step_mono :=
+      crashed_is_monotonic_in_one_step InitDelay GST MsgDelay
+        (tr (i + k)).s (tr (i + k + 1)).s (tr (i + k + 1)).a h_is_path
+    exact h_last_step_mono ik
+
 /--
   Every fair run covers every clock value `t`. Note that this requires fairness.
   Otherwise, the clock may not advance at all.
@@ -115,7 +149,7 @@ lemma eventually_clock_is_t
     specialize h_is_path (j - 1)
     unfold next_a at h_is_path
 
-    have h_jj: j - 1 + 1 = j := by omega;
+    have h_jj: j - 1 + 1 = j := by omega; -- JJ!
     rw [h_jj] at h_is_path -- replace `j - 1 + 1` with `j`
     have h_clock_advances_at_j: (tr j).a = Action.AdvanceClock := by simp [h_j_clock_advances]
     simp [h_clock_advances_at_j, advance_clock] at h_is_path
@@ -139,6 +173,67 @@ lemma eventually_crashes_stabilize
           C ⊆ (tr 0).s.all ∧ (tr (i + k)).s.crashed = C := by
   -- We could apply the fixpoint theorem to prove this,
   -- but I have not found a good instance of it in Mathlib4 yet.
+  sorry
+
+lemma eventually_alive_is_empty
+    (tr: Trace Proc)
+    (h_is_fair_run: is_fair_run Proc InitDelay GST MsgDelay tr)
+    (p: Proc)
+    (h_p_never_crashes: never_crashes tr p) (i: ℕ)
+    (h_i_positive: i > 0):
+      ∃ k: ℕ, (tr (i + k)).s.alive[p]! = ∅ := by
+  rcases h_is_fair_run with
+    ⟨ h_is_run, h_is_rel_comm, h_is_fair_to, h_is_fair_clock ⟩
+  unfold is_fair_timeout at h_is_fair_to
+  specialize h_is_fair_to i p
+  rcases h_is_fair_to with ⟨ j, h_j_clock_ge ⟩
+  -- this is the point when `p` triggers next timeout
+  specialize h_p_never_crashes (i + j - 1)
+  simp [h_p_never_crashes] at h_j_clock_ge
+  rcases h_j_clock_ge with ⟨ h_timeout, h_clock_at_timeout ⟩
+  unfold is_run at h_is_run
+  rcases h_is_run with ⟨ _, h_is_path ⟩
+  unfold is_path at h_is_path
+  specialize h_is_path (i + j - 1)
+  have h_dec_inc: i + j - 1 + 1 = i + j := by omega
+  rw [h_dec_inc, h_timeout] at h_is_path
+  unfold next_a at h_is_path
+  simp at h_is_path
+  unfold timeout at h_is_path
+  -- extract the update of the set `alive[p]!`
+  rcases h_is_path with ⟨ _, _, _, _, _, h_alive_updated, _ ⟩
+  have h_alive_is_empty: (tr (i + j)).s.alive[p]! = ∅ := by
+    simp [h_alive_updated]
+  exact ⟨ j, h_alive_is_empty ⟩
+
+/--
+  For every fair run, if `p` never crashes and `q` does,
+  then `p` never registers `q` as alive from some point on.
+  -/
+lemma eventually_crashes_implies_never_alive
+    (tr: Trace Proc)
+    (h_is_fair_run: is_fair_run Proc InitDelay GST MsgDelay tr)
+    (p q: Proc)
+    (h_p_never_crashes: never_crashes tr p)
+    (h_crashes: eventually_crashes tr q):
+      eventually_never_alive tr p q := by
+  -- eventually, `q` crashes at some point `at_q_crashed`
+  unfold eventually_crashes at h_crashes
+  rcases h_crashes with ⟨ at_q_crashed, h_q_crashed ⟩
+  -- Yet, `p` may still receive heartbeats from `q` from the past.
+  -- We jump to the point when `q` crashes and the pre-GST heartbeats stop arriving.
+  let beyond_gst := max (GST + MsgDelay + 1) (at_q_crashed + MsgDelay + 1)
+  -- eventually, `alive[p]!` becomes empty, we start with `beyond_gst`
+  have h_alive_is_empty :=
+    eventually_alive_is_empty InitDelay GST MsgDelay
+      tr h_is_fair_run p h_p_never_crashes beyond_gst
+  have h_positive: beyond_gst > 0 := by unfold beyond_gst; omega
+  simp [h_positive] at h_alive_is_empty
+  rcases h_alive_is_empty with ⟨ at_alive_empty, h_alive_empty ⟩
+  -- At this timepoint we have:
+  --   (1) `alive[p]! = ∅`,
+  --   (2) no pre-GST heartbeats from `q` can arrive
+  --   (3) `q` has crashed and no heartbeats from the previous timeout can arrive.
   sorry
 
 /--
